dist/Klas_GEMM_Naive1.cu
@@ -25,8 +25,10 @@ Klas_GEMM_Naive1_g_matmul_f32_rrr(uint32_t m,
                                   uint32_t n,
                                   uint32_t k, float *gA, float *gB, float *gC)
 {
-    KPR_KCALL(__hoisted_g_matmul_f32_rrr_0, m * n, 1U, 0U, n, k, gA, gB, gC);
-    MUST(cudaDeviceSynchronize());
+    cudaStream_t s = KPR_FRESH_STREAM();
+    KPR_KCALL(__hoisted_g_matmul_f32_rrr_0, m * n, 1U, 0U, s, n, k, gA, gB, gC);
+    MUST(cudaStreamSynchronize(s));
+    MUST(cudaStreamDestroy(s));
 }
 
 __global__
@@ -54,8 +56,10 @@ Klas_GEMM_Naive1_g_matmul_f64_rrr(uint32_t m,
                                   uint32_t k,
                                   double *gA, double *gB, double *gC)
 {
-    KPR_KCALL(__hoisted_g_matmul_f64_rrr_0, m * n, 1U, 0U, n, k, gA, gB, gC);
-    MUST(cudaDeviceSynchronize());
+    cudaStream_t s = KPR_FRESH_STREAM();
+    KPR_KCALL(__hoisted_g_matmul_f64_rrr_0, m * n, 1U, 0U, s, n, k, gA, gB, gC);
+    MUST(cudaStreamSynchronize(s));
+    MUST(cudaStreamDestroy(s));
 }
 
 __global__
@@ -83,8 +87,10 @@ Klas_GEMM_Naive1_g_matmul_u32_rrr(uint32_t m,
                                   uint32_t k,
                                   uint32_t *gA, uint32_t *gB, uint32_t *gC)
 {
-    KPR_KCALL(__hoisted_g_matmul_u32_rrr_0, m * n, 1U, 0U, n, k, gA, gB, gC);
-    MUST(cudaDeviceSynchronize());
+    cudaStream_t s = KPR_FRESH_STREAM();
+    KPR_KCALL(__hoisted_g_matmul_u32_rrr_0, m * n, 1U, 0U, s, n, k, gA, gB, gC);
+    MUST(cudaStreamSynchronize(s));
+    MUST(cudaStreamDestroy(s));
 }
 
 __global__
@@ -112,8 +118,10 @@ Klas_GEMM_Naive1_g_matmul_u64_rrr(uint32_t m,
                                   uint32_t k,
                                   uint64_t *gA, uint64_t *gB, uint64_t *gC)
 {
-    KPR_KCALL(__hoisted_g_matmul_u64_rrr_0, m * n, 1U, 0U, n, k, gA, gB, gC);
-    MUST(cudaDeviceSynchronize());
+    cudaStream_t s = KPR_FRESH_STREAM();
+    KPR_KCALL(__hoisted_g_matmul_u64_rrr_0, m * n, 1U, 0U, s, n, k, gA, gB, gC);
+    MUST(cudaStreamSynchronize(s));
+    MUST(cudaStreamDestroy(s));
 }
 
 __global__
@@ -141,8 +149,11 @@ Klas_GEMM_Naive1_g_matmul_f32_ccc(uint32_t m,
                                   uint32_t n,
                                   uint32_t k, float *gA, float *gB, float *gC)
 {
-    KPR_KCALL(__hoisted_g_matmul_f32_ccc_0, m * n, 1U, 0U, m, n, k, gA, gB, gC);
-    MUST(cudaDeviceSynchronize());
+    cudaStream_t s = KPR_FRESH_STREAM();
+    KPR_KCALL(__hoisted_g_matmul_f32_ccc_0, m * n, 1U, 0U, s, m, n, k, gA, gB,
+              gC);
+    MUST(cudaStreamSynchronize(s));
+    MUST(cudaStreamDestroy(s));
 }
 
 __global__
@@ -171,8 +182,11 @@ Klas_GEMM_Naive1_g_matmul_f64_ccc(uint32_t m,
                                   uint32_t k,
                                   double *gA, double *gB, double *gC)
 {
-    KPR_KCALL(__hoisted_g_matmul_f64_ccc_0, m * n, 1U, 0U, m, n, k, gA, gB, gC);
-    MUST(cudaDeviceSynchronize());
+    cudaStream_t s = KPR_FRESH_STREAM();
+    KPR_KCALL(__hoisted_g_matmul_f64_ccc_0, m * n, 1U, 0U, s, m, n, k, gA, gB,
+              gC);
+    MUST(cudaStreamSynchronize(s));
+    MUST(cudaStreamDestroy(s));
 }
 
 __global__
@@ -202,8 +216,11 @@ Klas_GEMM_Naive1_g_matmul_u32_ccc(uint32_t m,
                                   uint32_t k,
                                   uint32_t *gA, uint32_t *gB, uint32_t *gC)
 {
-    KPR_KCALL(__hoisted_g_matmul_u32_ccc_0, m * n, 1U, 0U, m, n, k, gA, gB, gC);
-    MUST(cudaDeviceSynchronize());
+    cudaStream_t s = KPR_FRESH_STREAM();
+    KPR_KCALL(__hoisted_g_matmul_u32_ccc_0, m * n, 1U, 0U, s, m, n, k, gA, gB,
+              gC);
+    MUST(cudaStreamSynchronize(s));
+    MUST(cudaStreamDestroy(s));
 }
 
 __global__
@@ -233,8 +250,11 @@ Klas_GEMM_Naive1_g_matmul_u64_ccc(uint32_t m,
                                   uint32_t k,
                                   uint64_t *gA, uint64_t *gB, uint64_t *gC)
 {
-    KPR_KCALL(__hoisted_g_matmul_u64_ccc_0, m * n, 1U, 0U, m, n, k, gA, gB, gC);
-    MUST(cudaDeviceSynchronize());
+    cudaStream_t s = KPR_FRESH_STREAM();
+    KPR_KCALL(__hoisted_g_matmul_u64_ccc_0, m * n, 1U, 0U, s, m, n, k, gA, gB,
+              gC);
+    MUST(cudaStreamSynchronize(s));
+    MUST(cudaStreamDestroy(s));
 }
 
 __global__
@@ -267,9 +287,11 @@ Klas_GEMM_Naive1_batched_matmul_f32(uint32_t batch,
                                     uint32_t n,
                                     uint32_t k, float *a, float *b, float *c)
 {
-    KPR_KCALL(__hoisted_batched_matmul_f32_0, batch * m * n, 1U, 0U, batch, m,
-              n, k, a, b, c);
-    MUST(cudaDeviceSynchronize());
+    cudaStream_t s = KPR_FRESH_STREAM();
+    KPR_KCALL(__hoisted_batched_matmul_f32_0, batch * m * n, 1U, 0U, s, batch,
+              m, n, k, a, b, c);
+    MUST(cudaStreamSynchronize(s));
+    MUST(cudaStreamDestroy(s));
 }
 
 __global__
@@ -295,9 +317,9 @@ __hoisted_batched_gemm_f32_0(float alpha,
         sum +=
             a[page * m * k + trow * k + vk] * b[page * k * n + vk * n + tcol];
     }
-    float s = sum;
+    float s1 = sum;
     c[page * m * n + trow * n + tcol] =
-        beta * c[page * m * n + trow * n + tcol] + alpha * s;
+        beta * c[page * m * n + trow * n + tcol] + alpha * s1;
 }
 
 void
@@ -308,7 +330,9 @@ Klas_GEMM_Naive1_batched_gemm_f32(float alpha,
                                   uint32_t n,
                                   uint32_t k, float *a, float *b, float *c)
 {
+    cudaStream_t s = KPR_FRESH_STREAM();
     KPR_KCALL(__hoisted_batched_gemm_f32_0,
-              batch * m * n, 1U, 0U, alpha, beta, batch, m, n, k, a, b, c);
-    MUST(cudaDeviceSynchronize());
+              batch * m * n, 1U, 0U, s, alpha, beta, batch, m, n, k, a, b, c);
+    MUST(cudaStreamSynchronize(s));
+    MUST(cudaStreamDestroy(s));
 }
