dist/Kuiper_Example_Polymorphism1.cu
@@ -23,8 +23,10 @@ void Kuiper_Example_Polymorphism1_swap_U64(uint64_t *r1, uint64_t *r2)
     uint64_t *gr2 = (uint64_t *) KPR_GPU_ALLOC(sizeof(uint64_t), 1U);
     MUST(cudaMemcpy(gr1, r1, sizeof(uint64_t), cudaMemcpyHostToDevice));
     MUST(cudaMemcpy(gr2, r2, sizeof(uint64_t), cudaMemcpyHostToDevice));
-    KPR_KCALL(__hoisted_swap_U64_0, 1U, 1U, 0U, gr1, gr2);
-    MUST(cudaDeviceSynchronize());
+    cudaStream_t s = KPR_FRESH_STREAM();
+    KPR_KCALL(__hoisted_swap_U64_0, 1U, 1U, 0U, s, gr1, gr2);
+    MUST(cudaStreamSynchronize(s));
+    MUST(cudaStreamDestroy(s));
     MUST(cudaMemcpy(r1, gr1, sizeof(uint64_t), cudaMemcpyDeviceToHost));
     MUST(cudaMemcpy(r2, gr2, sizeof(uint64_t), cudaMemcpyDeviceToHost));
     MUST(cudaFree(gr1));
@@ -53,8 +55,10 @@ void Kuiper_Example_Polymorphism1_swap_F32(float *r1, float *r2)
     float *gr2 = (float *)KPR_GPU_ALLOC(sizeof(float), 1U);
     MUST(cudaMemcpy(gr1, r1, sizeof(float), cudaMemcpyHostToDevice));
     MUST(cudaMemcpy(gr2, r2, sizeof(float), cudaMemcpyHostToDevice));
-    KPR_KCALL(__hoisted_swap_F32_0, 1U, 1U, 0U, gr1, gr2);
-    MUST(cudaDeviceSynchronize());
+    cudaStream_t s = KPR_FRESH_STREAM();
+    KPR_KCALL(__hoisted_swap_F32_0, 1U, 1U, 0U, s, gr1, gr2);
+    MUST(cudaStreamSynchronize(s));
+    MUST(cudaStreamDestroy(s));
     MUST(cudaMemcpy(r1, gr1, sizeof(float), cudaMemcpyDeviceToHost));
     MUST(cudaMemcpy(r2, gr2, sizeof(float), cudaMemcpyDeviceToHost));
     MUST(cudaFree(gr1));
