src/lib/kuiper/Kuiper.Epoch.fsti
@@ -2,19 +2,20 @@ module Kuiper.Epoch
 #lang-pulse
 
 open Pulse
+open Kuiper.Kernel.Stream
 
-type epoch_t = erased nat
+type epoch_t (s: stream_t) = erased nat
 
-val epoch_live (n:epoch_t) : slprop
-val epoch_done (n:epoch_t) : slprop
-
-ghost
-fn get_epoch ()
-  returns e : epoch_t
-  ensures epoch_live e
+val epoch_live (#s: stream_t) (n:epoch_t s) : slprop
+val epoch_done (#s: stream_t) (n:epoch_t s) : slprop
 
 ghost
-fn done_lower (e f : epoch_t)
-  preserves epoch_done e
+fn get_epoch (s: stream_t) ()
+  returns e : epoch_t s
+  ensures epoch_live #s e
+
+ghost
+fn done_lower (s: stream_t) (e f : epoch_t s)
+  preserves epoch_done #s e
   requires pure (f <= e)
-  ensures  epoch_done f
+  ensures  epoch_done #s f
