src/lib/kuiper/Kuiper.Kernel.Base.fsti
@@ -9,6 +9,9 @@ open Kuiper.Array
 open Kuiper.Epoch
 open Pulse.Lib.Pledge
 open Kuiper.Kernel.Desc
+open Kuiper.Kernel.Stream
+
+module SZ = Kuiper.SizeT
 
 (* This is the single primitive for launching kernels, with the most general
 type and capabilities. There are many simpler versions in the Kuiper.Kernel module,
@@ -18,22 +21,57 @@ fn launch_kernel_full
   (#full_pre : slprop)
   (#full_post : slprop)
   (k : kernel_desc full_pre full_post)
-  (#e : epoch_t)
-  preserves cpu
-  preserves epoch_live e
+  (s: stream_t)
+  (#e : epoch_t s)
+  preserves cpu ** stream_live s ** epoch_live e
   requires
     on gpu_loc full_pre
   ensures
     pledge0 (epoch_done e) (on gpu_loc full_post)
 
-(* Sync the device: wait for all pending kernels. *)
 noextract
-fn sync_device () (#e:epoch_t)
+fn sync_stream
+  (s: stream_t)
+  (#e:epoch_t s)
+  preserves
+    cpu ** stream_live s
   requires
     epoch_live e
   returns
-    e' : epoch_t
+    e' : epoch_t s
   ensures
     epoch_done e **
     epoch_live e' **
     pure (e' >= e)
+
+val sync_token: slprop
+
+ghost fn sync_stream_ghost
+  (s: stream_t)
+  (#e:epoch_t s)
+  preserves
+    sync_token ** stream_live s
+  requires
+    epoch_live e
+  returns
+    e' : epoch_t s
+  ensures
+    epoch_done e **
+    epoch_live e' **
+    pure (e' >= e)
+
+noextract
+fn sync_device ()
+  (frame: erased slprop)
+  (p: erased slprop)
+  (q: erased slprop)
+  (justif: 
+    ghost fn ()
+      preserves sync_token
+      requires frame ** p
+      ensures frame ** q)
+  preserves
+    frame ** cpu
+  requires p
+  ensures q
+
